Change to Clight in Blame. State additional invariants that are to be used when executing the context

security/Blame.v
@@ -1,8 +1,8 @@
 Require Import String.
-Require Import Coqlib Maps Errors.
+Require Import Coqlib Maps Errors Integers.
 Require Import AST Linking Smallstep Events Behaviors Memory Values.
 
-Require Import Csyntax Ctypes Ctyping Csem.
+Require Import Ctypes Cop Clight.
 Require Import Split.
 
 Definition same_domain (s: split) (j: meminj) (m: mem): Prop :=
@@ -22,32 +22,47 @@ Section Equivalence.
 Fixpoint remove_until_right (k: cont) :=
   match k with
   | Kstop => Kstop
-  | Kseq s k' => remove_until_right k'
-  | Kcall f en ctx ty k' =>
+  | Kseq _ k' | Kloop1 _ _ k'  | Kloop2 _ _ k' | Kswitch k' => remove_until_right k'
+  | Kcall id f en le k' =>
       match s (comp_of f) with
-      | Right => (* keep_until_left *) k
+      | Right => k
       | Left => remove_until_right k'
       end
-  | _ => Kstop (* TODO!! *)
   end.
-    (* with *)
-    (* keep_until_left (k: cont) := *)
-    (*   match k with *)
-    (*   | Kseq s k' => Kseq s (keep_until_left k') *)
-    (*   | *)
 
 Inductive right_cont_injection: cont -> cont -> Prop :=
 | right_cont_injection_kstop: right_cont_injection Kstop Kstop
 | right_cont_injection_kseq: forall s k1 k2,
     right_cont_injection k1 k2 ->
     right_cont_injection (Kseq s k1) (Kseq s k2) (* TODO: write other cases *)
-| right_cont_injection_kcall_left: forall f1 f2 en1 en2 ctx1 ctx2 ty1 ty2 k1 k2,
+| right_cont_injection_kloop1: forall s s' k1 k2,
+    right_cont_injection k1 k2 ->
+    right_cont_injection (Kloop1 s s' k1) (Kloop1 s s' k2)
+| right_cont_injection_kloop2: forall s s' k1 k2,
+    right_cont_injection k1 k2 ->
+    right_cont_injection (Kloop2 s s' k1) (Kloop2 s s' k2)
+| right_cont_injection_kswitch: forall k1 k2,
+    right_cont_injection k1 k2 ->
+    right_cont_injection (Kswitch k1) (Kswitch k2)
+| right_cont_injection_kcall_left: forall id1 id2 f1 f2 en1 en2 le1 le2 k1 k2,
     s (comp_of f1) = Left ->
     s (comp_of f2) = Left ->
     right_cont_injection (remove_until_right k1) (remove_until_right k2) ->
-      (* might be the same type?*)
-    right_cont_injection (Kcall f1 en1 ctx1 ty1 k1) (Kcall f2 en2 ctx2 ty2 k2)
+    right_cont_injection (Kcall id1 f1 en1 le1 k1) (Kcall id2 f2 en2 le2 k2)
 .
+
+Definition right_env_injection (e1 e2: env): Prop :=
+  forall i b ty,
+    e1 ! i = Some (b, ty) ->
+    exists b', j b = Some (b', 0%Z) /\
+          e2 ! i = Some (b', ty).
+
+Definition right_tenv_injection (le1 le2: temp_env): Prop :=
+  forall i v,
+    le1 ! i = Some v ->
+    exists v', Val.inject j v v' /\
+            le2 ! i = Some v'.
+
 
  (* Analogous to: [partialize ctx scs1 = partialize ctx scs2] with
     [ctx] giving us the [Left] part (the program part). Partialize keeps the context part
@@ -57,7 +72,7 @@ Inductive right_cont_injection: cont -> cont -> Prop :=
   the program part of the two states.
   *)
 Variant right_executing_injection: state -> state -> Prop :=
-| inject_states: forall f s k1 k2 en m1 m2,
+| inject_states: forall f s k1 k2 e1 e2 le1 le2 m1 m2,
     (* we forget about program memories but require injection of context memories *)
     right_mem_injection m1 m2 ->
 
@@ -65,16 +80,11 @@ Variant right_executing_injection: state -> state -> Prop :=
        context continuation *)
     right_cont_injection k1 k2 ->
 
-    right_executing_injection (State f s k1 en m1) (State f s k2 en m2)
-| inject_exprstates: forall f e k1 k2 en m1 m2,
-    (* we forget about program memories but require injection of context memories *)
-    right_mem_injection m1 m2 ->
+    (* the environments satisfy the injection *)
+    right_env_injection e1 e2 ->
+    right_tenv_injection le1 le2 ->
 
-    (* we forget about program parts of the continuation but require injection of
-       context continuation *)
-    right_cont_injection k1 k2 ->
-
-    right_executing_injection (ExprState f e k1 en m1) (ExprState f e k2 en m2)
+    right_executing_injection (State f s k1 e1 le1 m1) (State f s k2 e2 le2 m2)
 | inject_callstates: forall f vs k1 k2 m1 m2,
     (* we forget about program memories but require injection of context memories *)
     right_mem_injection m1 m2 ->
@@ -93,8 +103,7 @@ Variant right_executing_injection: state -> state -> Prop :=
     right_cont_injection k1 k2 ->
 
     right_executing_injection (Returnstate v k1 m1 ty cp) (Returnstate v k2 m2 ty cp)
-| inject_stuckstates:
-    right_executing_injection Stuckstate Stuckstate.
+.
 
 Axiom is_left: split -> state -> Prop.
 Axiom is_right: split -> state -> Prop.
@@ -127,35 +136,162 @@ Variant right_state_injection: state -> state -> Prop :=
 End Equivalence.
 
 Section Simulation.
-  Context (c p1 p2: Csyntax.program).
+  Context (c p1 p2: Clight.program).
   Variable s: split.
   Variable j: meminj.
 
   Context (ge1 ge2: genv).
 
+  Lemma eval_expr_lvalue_injection:
+    forall s j m1 m2 e1 e2 le1 le2 cp,
+    forall inj: right_mem_injection s j m1 m2,
+    forall env_inj: right_env_injection j e1 e2,
+    forall lenv_inj: right_tenv_injection j le1 le2,
+    (forall a v,
+      eval_expr ge1 e1 cp le1 m1 a v ->
+      (* forall loc ofs (EQv: v = Vptr loc ofs), *)
+      exists v', Val.inject j v v' /\
+                     eval_expr ge2 e2 cp le2 m2 a v')
+      /\
+    (forall a loc ofs bf,
+      eval_lvalue ge1 e1 cp le1 m1 a loc ofs bf ->
+      exists loc' ofs', j loc = Some (loc', ofs') /\
+                     eval_lvalue ge2 e2 cp le2 m2 a loc' (Ptrofs.add ofs (Ptrofs.repr ofs')) bf).
+  Proof.
+    intros.
+    destruct inj as [inj_dom inj_inject].
+    apply eval_expr_lvalue_ind; intros;
+    try now match goal with
+    | |- exists _, Val.inject _ (Vint _) _ /\ _ => eexists; split; [eapply Val.inject_int | econstructor; eauto]
+    | |- exists _, Val.inject _ (Vfloat _) _ /\ _ => eexists; split; [eapply Val.inject_float | econstructor; eauto]
+    | |- exists _, Val.inject _ (Vsingle _) _ /\ _ => eexists; split; [eapply Val.inject_single | econstructor; eauto]
+    | |- exists _, Val.inject _ (Vlong _) _ /\ _ => eexists; split; [eapply Val.inject_long | econstructor; eauto]
+    end.
+    - exploit lenv_inj; eauto. intros [loc' [? ?]].
+      eexists; split; eauto.
+      constructor; auto.
+    - destruct H0 as [loc' [ofs' [? ?]]].
+      eexists; split; eauto.
+      econstructor; eauto.
+    - destruct H0 as [v' [? ?]].
+      exploit sem_unary_operation_inject; eauto.
+      intros [? [? ?]].
+      eexists; split; eauto.
+      econstructor; eauto.
+    - destruct H0 as [v1' [? ?]].
+      destruct H2 as [v2' [? ?]].
+      exploit sem_binary_operation_inject; eauto.
+      intros [? [? ?]].
+      eexists; split; eauto.
+      econstructor; eauto.
+    -
+    - (* this is a contradictory case: there is no unary operation that returns a pointer *)
+      destruct op; simpl in *.
+      + rewrite notbool_bool_val in H1.
+        destruct (bool_val _ _ _); [| congruence].
+        inv H1. now destruct b.
+      + unfold sem_notint in H1. destruct (classify_notint _); [| | congruence].
+        now destruct v1. now destruct v1.
+      + unfold sem_neg in H1. destruct (classify_neg _); try congruence; now destruct v1.
+      + unfold sem_absfloat in H1. destruct (classify_neg _); try congruence; now destruct v1.
+    - assert ((exists loc0 ofs0, v1 = Vptr loc0 ofs0) \/
+             (exists loc0 ofs0, v2 = Vptr loc0 ofs0)).
+      { destruct op; simpl in *.
+        - unfold sem_add in *.
+          destruct (classify_add _ _); simpl in *.
+          destruct v1, v2; simpl in *; destruct Archi.ptr64; simpl in *; inv H3; left; eexists; eexists; eauto.
+          destruct v1, v2; simpl in *; destruct Archi.ptr64; simpl in *; inv H3; left; eexists; eexists; eauto.
+          destruct v1, v2; simpl in *; destruct Archi.ptr64; simpl in *; inv H3; right; eexists; eexists; eauto.
+          destruct v1, v2; simpl in *; destruct Archi.ptr64; simpl in *; inv H3; right; eexists; eexists; eauto.
+          destruct (typeof a1), (typeof a2); unfold sem_binarith in *; simpl in *; try now inv H3.
+          destruct v1, v2; simpl in *.
+          unfold sem_binarith.
+
+
+            try (now
+              destruct v1, v2; simpl in *; destruct Archi.ptr64; simpl in *; inv H3; try (left; eexists; eexists; eauto);
+               try (right; eexists; eexists; eauto)).
+
+          destruct v2, v1; simpl in *; destruct Archi.ptr64; inv H3.
+            try now (eexists; eexists; eauto).
+
+            eexists; eexists; eauto.
+          + destruct v1, v2; simpl in *; destruct Archi.ptr64; simpl in *; inv H3.
+            eexists; eexists; eauto.
+            eexists; eexists; eauto.
+          +
+            simpl in H3.
+          destruct v1. simpl in H3.
+            try now destruct v1.
+          destruct v1; try now auto.
+
+        - rewrite notbool_bool_val in H1.
+          destruct (bool_val _ _ _); [| congruence].
+          inv H1. now destruct b.
+        - unfold sem_notint in H1. destruct (classify_notint _); [| | congruence].
+          now destruct v1. now destruct v1.
+        - unfold sem_neg in H1. destruct (classify_neg _); try congruence; now destruct v1.
+        - unfold sem_absfloat in H1. destruct (classify_neg _); try congruence; now destruct v1. }
+      subst v1.
+      specialize (H0 _ _ eq_refl) as [loc' [ofs' [? ?]]].
+      (* exploit sem_unary_operation_inject; eauto. *)
+      (* intros [tv [? ?]]. *)
+      (* destruct tv; try now inv H4. *)
+      (* inv H4. *)
+      exists loc', ofs'; split; eauto.
+      econstructor; eauto.
+      rewrite H3. congruence.
+    -
+
 
   Lemma parallel_concrete: forall s1 s2 s1' t,
       right_state_injection s j s1 s2 ->
       is_right s s1 ->
-      Csem.step ge1 s1 t s1' ->
+      Clight.step1 ge1 s1 t s1' ->
       exists s2',
-        Csem.step ge2 s2 t s2' /\
+        Clight.step1 ge2 s2 t s2' /\
           right_state_injection s j s1' s2'.
     Proof.
       intros s1 s2 s1' t rs_inj is_r step1.
       inv rs_inj.
       - admit. (* contradiction *)
-      - inv step1; inv H2.
-        + inv H1.
-          assert (lemma: right_mem_injection s j m m2 ->
-                  lred ge1 e a m a' m' ->
-                  exists m2', lred ge2 e a m2 a' m2' /\ right_mem_injection s j m' m2').
-          admit.
-          exploit lemma; eauto. intros [? [? ?]].
+      - inv step1; inv H1.
+        + assert (lemma1:
+                   right_mem_injection s j m m2 ->
+                   right_env_injection j e e2 ->
+                   right_tenv_injection j le le2 ->
+                   eval_lvalue ge1 e (comp_of f) le m a1 loc ofs bf ->
+                   exists loc' ofs', j loc = Some (loc', ofs') /\
+                          eval_lvalue ge2 e2 (comp_of f) le2 m2 a1 loc' (Ptrofs.add ofs (Ptrofs.repr ofs')) bf).
+          { clear.
+            intros inj env_inj lenv_inj ev.
+            destruct inj as [inj_dom inj_inject].
+            inv ev.
+            - exploit env_inj; eauto. intros [loc' [? ?]].
+              exists loc', 0%Z. split; eauto.
+              constructor; eauto.
+            - admit.
+            - eexists; eexists; split; eauto. admit.
+              constructor. admit.
+
+              admit.
+            - admit.
+            - admit.
+          }
+          exploit lemma1; eauto.
+          intros [loc' [ofs' [? ?]]].
+
           eexists; split.
-          constructor. constructor; eauto.
-          right. admit. admit. econstructor; eauto.
-  Admitted.
+          econstructor. eauto.
+          intros [loc' [ofs' [? ?]]].
+          eassumption.
+
+
+          admit. admit. admit. admit.
+          right. admit. admit.
+          econstructor; eauto. admit.
+Admitted.
+
 
     (* Example that shows why Blame doesn't hold in the C semantics.
        Because the semantics are not determinate we can end up in situation like this one:
